thy/Iptables_Semantics/Semantics_Ternary/MatchExpr_Fold.thy
@@ -1,0 +1,67 @@
+section\<open>Combine Match Expressions\<close>
+theory MatchExpr_Fold
+imports Primitive_Normalization
+begin
+
+fun andfold_MatchExp :: "'a match_expr list \<Rightarrow> 'a match_expr" where
+  "andfold_MatchExp [] = MatchAny" |
+  "andfold_MatchExp [e] = e" |
+  "andfold_MatchExp (e#es) = MatchAnd e (andfold_MatchExp es)"
+
+lemma andfold_MatchExp_alist_and: "alist_and' (map Pos ls) = andfold_MatchExp (map Match ls)"
+  apply(induction ls)
+   apply(simp)
+  apply(simp)
+  apply(rename_tac l ls)
+  apply(case_tac "ls")
+   by(simp)+
+
+lemma andfold_MatchExp_matches:
+  "matches \<gamma> (andfold_MatchExp ms) a p \<longleftrightarrow> (\<forall>m \<in> set ms. matches \<gamma> m a p)"
+  apply(induction ms rule: andfold_MatchExp.induct)
+    apply(simp add: bunch_of_lemmata_about_matches)+
+  done
+
+lemma andfold_MatchExp_not_discI:
+  "\<forall>m \<in> set ms. \<not> has_disc disc m \<Longrightarrow> \<not> has_disc disc (andfold_MatchExp ms)"
+  by(induction ms rule: andfold_MatchExp.induct) (simp)+
+
+lemma andfold_MatchExp_not_disc_negatedI:
+  "\<forall>m \<in> set ms. \<not> has_disc_negated disc False m \<Longrightarrow> \<not> has_disc_negated disc False (andfold_MatchExp ms)"
+  by(induction ms rule: andfold_MatchExp.induct) (simp)+
+
+lemma andfold_MatchExp_not_disc_negated_mapMatch:
+  "\<not> has_disc_negated disc False (andfold_MatchExp (map (Match \<circ> C) ls))"
+  apply(induction ls)
+   apply(simp; fail)
+  apply(simp)
+   apply(rename_tac ls, case_tac ls)
+  by(simp)+
+
+lemma andfold_MatchExp_not_disc_mapMatch:
+  "\<forall>a. \<not> disc (C a) \<Longrightarrow> \<not> has_disc disc (andfold_MatchExp (map (Match \<circ> C) ls))"
+  apply(induction ls)
+   apply(simp; fail)
+  apply(simp)
+   apply(rename_tac ls, case_tac ls)
+  by(simp)+
+
+lemma andfold_MatchExp_normalized_nnf: "\<forall>m \<in> set ms. normalized_nnf_match m \<Longrightarrow>
+    normalized_nnf_match (andfold_MatchExp ms)"
+  by(induction ms rule: andfold_MatchExp.induct)(simp)+
+
+lemma andfold_MatchExp_normalized_n_primitive: "\<forall>m \<in> set ms. normalized_n_primitive (disc, sel) f m \<Longrightarrow>
+    normalized_n_primitive (disc, sel) f (andfold_MatchExp ms)"
+  by(induction ms rule: andfold_MatchExp.induct)(simp)+
+
+lemma andfold_MatchExp_normalized_normalized_n_primitive_single:
+    "\<forall>a. \<not> disc (C a) \<Longrightarrow>
+      s \<in> set (normalize_match (andfold_MatchExp (map (Match \<circ> C) xs))) \<Longrightarrow>
+         normalized_n_primitive (disc, sel) f s"
+  apply(rule normalized_n_primitive_if_no_primitive)
+   using normalized_nnf_match_normalize_match apply blast
+  apply(rule normalize_match_preserves_nodisc[where m="(andfold_MatchExp (map (Match \<circ> C) xs))"])
+   apply simp_all
+  by (simp add: andfold_MatchExp_not_discI)
+
+end
